src/program_logic/na_crash_inv.v
@@ -19,8 +19,8 @@ Implicit Types Φc : iProp Σ.
 Implicit Types v : val Λ.
 Implicit Types e : expr Λ.
 
-Definition na_crash_inv_def N k Q P :=
-  (∃ γ Q0 Qr, staged_value k (N.@"1") (N.@"2") (⊤ ∖ ↑N.@"1" ∖ ↑N.@"2") γ Q0 Qr P ∗ (Q0 -∗ Q) ∗ ▷ □ (Q -∗ P))%I.
+Definition na_crash_inv_def k Q P :=
+  (∃ γ Q0 Qr, staged_value k O O ⊤ γ Q0 Qr P ∗ (Q0 -∗ Q) ∗ ▷ □ (Q -∗ P))%I.
 Definition na_crash_inv_aux : seal (@na_crash_inv_def). by eexists. Qed.
 Definition na_crash_inv := (na_crash_inv_aux).(unseal).
 Definition na_crash_inv_eq := (na_crash_inv_aux).(seal_eq).
@@ -30,13 +30,12 @@ Ltac crash_unseal :=
   rewrite ?na_crash_inv_eq;
   rewrite /na_crash_inv_def.
 
-Lemma na_crash_inv_alloc N k E P Q:
-  ↑N ⊆ E →
-  ▷ Q -∗ ▷ □ (Q -∗ P) -∗ |(S k)={E}=> na_crash_inv N (S k) Q P ∗ <disc> |C={⊤, ∅}_(S k)=> P.
+Lemma na_crash_inv_alloc k E P Q:
+  ▷ Q -∗ ▷ □ (Q -∗ P) -∗ |(S k)={E}=> na_crash_inv (S k) Q P ∗ <disc> |C={⊤, ∅}_(S k)=> P.
 Proof.
   crash_unseal.
-  iIntros (?) "HQ #HQP".
-  iMod (staged_inv_alloc (k) (N.@"1") (N.@"2") E (⊤ ∖ ↑N.@"1" ∖ ↑N.@"2")
+  iIntros "HQ #HQP".
+  iMod (staged_inv_alloc (k) E ⊤
                          P Q True%I with "[HQ]") as (i') "(#Hinv&Hval&Hpend)".
   { iFrame "#". iFrame. iModIntro; iIntros; eauto. iSplitL; last done.
     iApply "HQP"; eauto. }
@@ -44,19 +43,18 @@ Proof.
   iSplitL "Hval".
   { iExists _, Q, _. iFrame. iFrame "#". auto. }
   iApply (staged_inv_init_cfupd' with "[Hpend]"); eauto.
-  solve_ndisj.
 Qed.
 
-Lemma na_crash_inv_status_wand N k Q P:
-  na_crash_inv N k Q P -∗
+Lemma na_crash_inv_status_wand k Q P:
+  na_crash_inv k Q P -∗
   ▷ □ (Q -∗ P).
 Proof. crash_unseal. iDestruct 1 as (???) "(?&?&$)". Qed.
 
-Lemma na_crash_inv_weaken N k Q Q' P :
+Lemma na_crash_inv_weaken k Q Q' P :
   (Q -∗ Q') -∗
   ▷ □(Q' -∗ P) -∗
-  na_crash_inv N k Q P -∗
-  na_crash_inv N k Q' P.
+  na_crash_inv k Q P -∗
+  na_crash_inv k Q' P.
 Proof.
   crash_unseal.
   iIntros "HQ' #HQ'P H".
@@ -65,31 +63,28 @@ Proof.
   iFrame "#". iIntros. iApply "HQ'". by iApply "Hwand0".
 Qed.
 
-Lemma wpc_na_crash_inv_open_modify Qnew s k k' k'' E1 E2 e Φ Φc Q P N :
-  ↑N ⊆ E1 →
+Lemma wpc_na_crash_inv_open_modify Qnew s k k' k'' E1 E2 e Φ Φc Q P :
   k'' ≤ k' →
   k'' ≤ (S k) →
-  na_crash_inv N (S k') Q P -∗
-  (<disc> ▷ Φc ∧ (▷ Q -∗ WPC e @ NotStuck; k''; (E1 ∖ ↑N); ∅
+  S k ≤ k' →
+  na_crash_inv (S k') Q P -∗
+  (<disc> ▷ Φc ∧ (▷ Q -∗ WPC e @ NotStuck; k''; E1; ∅
                     {{λ v, ▷ Qnew v ∗
-                           ▷ □ (Qnew v -∗ P)  ∗ (na_crash_inv N (S k') (Qnew v) P -∗ (<disc> ▷ Φc ∧ Φ v))}}
+                           ▷ □ (Qnew v -∗ P)  ∗ (na_crash_inv (S k') (Qnew v) P -∗ (<disc> ▷ Φc ∧ Φ v))}}
                     {{ Φc ∗ P }})) -∗
   WPC e @ s; (S k); E1; E2 {{ Φ }} {{ Φc }}.
 Proof.
   crash_unseal.
   iIntros (???) "Hbundle Hwp".
   iDestruct "Hbundle" as (???) "(Hval&HQ0&HQP)".
-  iApply (wpc_staged_inv_open' _ _ _ _ _ _ _ _ _ _ _ _ _ Qnew _ with "[-]"); try iFrame "Hval"; eauto.
-  { solve_ndisj. }
-  { solve_ndisj. }
-  { solve_ndisj. }
+  iApply (wpc_staged_inv_open' _ _ _ _ _ _ _ _ _ _ _ _ _ _ _ Qnew _ with "[-]"); try iFrame "Hval"; eauto.
+  { lia. }
   iSplit.
   { iDestruct "Hwp" as "($&_)". }
   iDestruct "Hwp" as "(_&Hwp)". iIntros "HQ".
   iSpecialize ("Hwp" with "[HQ0 HQ]").
   { iNext. iApply "HQ0". eauto. }
   iApply (wpc_strong_mono with "Hwp"); auto.
-  { solve_ndisj. }
   iSplit.
   - iIntros (?) "(HQ&#Hwand'&HQrest)".
     iModIntro. iFrame "HQ Hwand'". iIntros "Hval'".
@@ -99,19 +94,19 @@ Qed.
 
 (* TODO: in theory this can implement ElimAcc for iInv support; see
 [elim_acc_wp_nonatomic] *)
-Lemma wpc_na_crash_inv_open s k k' k'' E1 E2 e Φ Φc Q P N:
-  ↑N ⊆ E1 →
+Lemma wpc_na_crash_inv_open s k k' k'' E1 E2 e Φ Φc Q P:
   k'' ≤ k' →
   k'' ≤ (S k) →
-  na_crash_inv N (S k') Q P -∗
-  (<disc> ▷ Φc ∧ (▷ Q -∗ WPC e @ NotStuck; k''; (E1 ∖ ↑N); ∅
-                    {{λ v, ▷ Q ∗ (na_crash_inv N (S k') Q P -∗ (<disc> ▷ Φc ∧ Φ v))}}
+  S k ≤ k' →
+  na_crash_inv (S k') Q P -∗
+  (<disc> ▷ Φc ∧ (▷ Q -∗ WPC e @ NotStuck; k''; E1; ∅
+                    {{λ v, ▷ Q ∗ (na_crash_inv (S k') Q P -∗ (<disc> ▷ Φc ∧ Φ v))}}
                     {{ Φc ∗ P }})) -∗
   WPC e @ s; (S k); E1; E2 {{ Φ }} {{ Φc }}.
 Proof.
   iIntros (???) "H1 Hwp".
   iDestruct (na_crash_inv_status_wand with "H1") as "#Hwand".
-  iApply (wpc_na_crash_inv_open_modify with "[$] [Hwp]"); eauto.
+  iApply (wpc_na_crash_inv_open_modify _ s k k' k'' with "[$] [Hwp]"); eauto.
   iSplit.
   - iDestruct "Hwp" as "($&_)".
   - iIntros "HQ". iDestruct "Hwp" as "(_&Hwp)". iSpecialize ("Hwp" with "[$]").
@@ -120,10 +115,12 @@ Proof.
     * iModIntro. eauto.
 Qed.
 
+(* TODO, follows the pattern of staged_inv, the swap has to be atomic now *)
+(*
 Lemma na_crash_inv_open_modify N k' k E E' P Q R:
   ↑N ⊆ E →
   k' ≤ k →
-  na_crash_inv N (S k') Q P -∗
+  na_crash_inv (S k') Q P -∗
   ((▷ Q ∗ (∀ Q', ▷ Q' ∗ □ ▷ (Q' -∗ P) -∗ |(S k)={E∖↑N,E}=> na_crash_inv N (S k') Q' P)) ∨
    (C ∗ |(S k)={E∖↑N, E}=> na_crash_inv N (S k') Q P) -∗ |(S k)={E ∖ ↑N, E'}=> R) -∗
   (|(S k)={E,E'}=> R).
@@ -170,5 +167,6 @@ Proof.
    - iLeft. iDestruct "H1" as "($&H)". iIntros "HQ". by iMod ("H" $! Q with "[$]").
    - iRight. iFrame.
 Qed.
+*)
 
 End ci.
